Better modularization

coq/ServerLang.v
@@ -1,10 +1,16 @@
 Require Import Common.
 
+Require EqNat.
+
+Module Server <: ServerSem.
 
 Definition var := nat.
+Definition Env := var -> nat.
+
+Section Syntax.
 
 Inductive Cmd :=
-  | call (func v: var)
+  | call_coq (v: var) (coq: Env -> nat)
 .
 
 Inductive Method :=
@@ -13,49 +19,15 @@ Inductive Method :=
 
 Definition Prog := list Method.
 
-Definition var_car := 0.
-Definition var_door1 := 1.
-Definition var_goat := 2.
-Definition var_door2 := 3.
-Definition var_winner := 4.
-Definition var_hcar := 5.
-Definition var_compute_winner := 6.
+End Syntax.
 
-Definition receive_emit role var :=  proc role var [] var.
+Section Semantics.
 
-Definition host := 0.
-Definition guest := 1.
-
-Definition Monty := [
-  receive_emit host  var_hcar;
-  receive_emit guest var_door1;
-  receive_emit host  var_goat;
-  receive_emit guest var_door2;
-  receive_emit host  var_car;
-  proc guest 0 [call var_compute_winner var_winner] var_winner
-].
-
-Definition Env := var -> nat.
-Definition ServState: Set := Env * Prog.
-
-
-Definition guest_winner (hcar door1 goat door2 car : nat) : bool :=
-  negb (Nat.eqb hcar car)
-  || Nat.eqb car goat
-  || Nat.eqb goat door1
-  || Nat.eqb car door2
-  .
+Definition State: Set := Env * Prog.
 
 Definition server_eval_cmd (env: Env) (cmd: Cmd) : Env :=
   match cmd with
-  | call 6 v1 =>
-    let winner := 
-      if guest_winner (env var_hcar) (env var_door1) (env var_goat) (env var_door2) (env var_car) then
-        1
-      else
-        0
-    in (update env v1 winner)
-  | call _ v1 => env
+  | call_coq v cf => update env v (cf env)
   end
 .
 
@@ -65,7 +37,7 @@ Fixpoint server_eval_cmds (env: Env) (cmds: list Cmd) : Env :=
   | cmd::cmds => server_eval_cmds (server_eval_cmd env cmd) cmds
   end.
 
-Definition server_eval '(st, packet) : (ServState * Event) :=
+Definition eval '(st, packet) : (State * Event) :=
   let '(env, prog) := st in
   match (prog, packet) with
   | (proc expected v1 cmds v2 :: ms, mkPkt actual (M_nat m)) =>
@@ -80,26 +52,27 @@ Definition server_eval '(st, packet) : (ServState * Event) :=
   end
 .
 
-Require Import EqNat.
 
-Definition owns_client (client: nat) st :=
+Definition owns_user (client: nat) st :=
   forall actual content,
     actual = client \/
-      fst (server_eval (st, mkPkt actual content)) = st.
+      eval (st, mkPkt actual content) = (st, M_empty).
 
 Lemma owns_receiver : forall id lval cmd emit env ms,
-  owns_client id (env, proc id lval cmd emit::ms).
+  owns_user id (env, proc id lval cmd emit::ms).
 Proof.
-  unfold owns_client.
-  intros.
-  destruct (eq_nat_decide actual id).
-  * left. exact (eq_nat_eq actual id e).
-  * right. unfold not in n.
-    simpl.
-    destruct content; try reflexivity.
-    destruct (Nat.eqb actual id) eqn:EQ; try reflexivity.
+  unfold owns_user;
+  intros;
+  destruct (EqNat.eq_nat_decide actual id); [left | right].
+  * exact (EqNat.eq_nat_eq actual id e).
+  * simpl.
+    destruct content, (Nat.eqb actual id) eqn:BEQ; try reflexivity.
     exfalso.
-    apply beq_nat_true in EQ.
-    subst actual.
-    exact (n (eq_nat_refl id)).
+    apply EqNat.beq_nat_true in BEQ.
+    subst.
+    apply n, EqNat.eq_nat_refl.
 Qed.
+
+End Semantics.
+
+End Server.
