coq/ClientLang.v
@@ -1,5 +1,7 @@
 Require Import Common.
 
+Module Client <: ClientSem.
+
 Definition var := nat.
 
 
@@ -16,57 +18,13 @@ Inductive ClientCmd :=
 
 Definition Prog := list ClientCmd.
 
-(* example: Monty Hall *)
 
-Definition var_car := 0.
-Definition var_door1 := 1.
-Definition var_goat := 2.
-Definition var_door2 := 3.
-Definition var_winner := 4.
-Definition var_hcar := 5.
+Section Semantics.
 
-
-Definition mh_host : Prog := [
-  input var_car;
-  hash var_car var_hcar;
-  send var_hcar;
-  drop;
-  receive var_door1;
-  print var_door1;
-  input var_goat;
-  send var_goat;
-  drop;
-  receive var_door2;
-  print var_door2;
-  send var_car;
-  receive var_winner;
-  print var_winner
-].
-
-Definition mh_guest : Prog := [
-  receive var_hcar;
-  input var_door1;
-  send var_door1;
-  drop;
-  receive var_goat;
-  input var_door2;
-  send var_door2;
-  drop;
-  receive var_winner;
-  print var_winner
-].
-
-
-(* Semantics *)
 Definition Env := var -> nat.
-Record ClState : Set := mkSt {
-  Cenv: Env;
-  Cprog: Prog;
-  Clog_index: nat
-}.
+Definition State : Set :=  Env * Prog * nat.
 
-Section X.
-
+Section VariablesForInductive.
 Variables (env: Env) (n: nat) (log: option Event).
 
 (* As defined here, this requires FunctionalExtensionality on update env *)
@@ -83,12 +41,11 @@ Inductive client_cmd_step : ClientCmd -> Env * option Msg * nat -> Prop :=
   | is_input : forall lval x,
                 client_cmd_step (input lval) ((update env lval x), None, n)
 .
+End VariablesForInductive.
 
-End X.
-
-Definition client_step' (st: ClState) (log: list Event) (st': ClState) (m: option Msg) : Prop :=
-  let 'mkSt env prog logindex := st in
-  let 'mkSt env' prog' logindex' := st' in
+Definition client_step' (st: State) (log: list Event) (st': State) (m: option Msg) : Prop :=
+  let '(env, prog, logindex) := st in
+  let '(env', prog', logindex') := st' in
   match prog with
   | [] => False
   | cmd::cmds =>  prog' = cmds
@@ -96,15 +53,9 @@ Definition client_step' (st: ClState) (log: list Event) (st': ClState) (m: optio
   end
 .
 
-Definition client_step '(st, log) '(st', m) : Prop :=
-  client_step' st log st' m.
+Definition step : (State * list Event) -> (State * option Msg) -> Prop :=
+  fun '(st, log) '(st', m) => client_step' st log st' m.
 
-Definition init_env := (fun (x: var) => 0).
-Definition st := (mkSt init_env mh_host 0).
-Definition st' := (mkSt (update init_env var_car 0) (tail mh_host) 0).
+End Semantics.
 
-Example input_can_be_nop : (client_step' st [] st' None).
-  split.
-  * reflexivity.
-  * exact (is_input init_env 0 None var_car 0).
-Qed.
+End Client.
