coq/Common.v
@@ -11,7 +11,7 @@ Definition ClientId := nat.
 
 Definition Event: Set := Content.
 Definition Msg: Set := Content.
-Record State : Set := mkPkt {
+Record Packet : Set := mkPkt {
   sender: ClientId;
   msgof: Msg
 }.
@@ -20,3 +20,20 @@ Definition update {T: Type} f (id: nat) (v: T) id' :=
   if Nat.eqb id id' then v
   else f id.
 
+
+Module Type ServerSem.
+Parameter State: Set.
+Parameter eval : (State * Packet) -> (State * Event).
+End ServerSem.
+
+Module Type ClientSem.
+Parameter State: Set.
+Parameter step : (State * list Event) -> (State * option Msg) -> Prop.
+End ClientSem.
+
+
+Definition inject_cons {T} (x: option T) xs :=
+  match x with
+    | Some x => x::xs
+    | None => xs
+  end.
